First draft of the proof checker theory + certified clausal form normalization

theories/Proof.v
@@ -1,11 +1,105 @@
 Require Import Checker.Atomic.
+Require Import Checker.Linear.
+Require Import Checker.Nogood.
+Require Import Checker.Variable.
+Require Import Bool.
+Require Import List.
 
-Inductive Step :=
-  | inference (premises : list Atomic) (conclusion : Atomic).
+Inductive InferenceRule :=
+  | linear (constraint : LinearConstraint)
+  | rup_inf (database : list Clause).
 
+Record Step := 
+  {
+    premises : list Atomic ;
+    consequent : Atomic ;
+    inference_rule : InferenceRule ;
+  }.
+
+Definition clausal_form (step : Step) : Clause :=
+  (consequent step) :: (map atomic_not (premises step)).
+
+Definition satisfies_impl (x : Step) (sol : Assignment) :=
+  orb
+  (test_atomic_assignment (consequent x) sol)
+  (existsb (fun p : Atomic => negb (test_atomic_assignment p sol)) (premises x)).
+
+Theorem clausal_form_equiv : forall (step : Step) (sol : Assignment),
+  Is_true (satisfies_impl step sol) <-> Is_true (satisfies_nogood (clausal_form step) sol).
+Proof.
+  intros.
+  split.
+  - intros Himpl.
+    destruct (test_atomic_assignment (consequent step) sol) eqn:Eatomic ;
+    unfold clausal_form ;
+    unfold test_atomic_assignment in Eatomic ;
+    simpl ;
+    rewrite Eatomic ;
+    try reflexivity.
+    unfold satisfies_impl in Himpl.
+    unfold test_atomic_assignment in Himpl.
+    rewrite Eatomic in Himpl.
+    simpl in Himpl.
+    apply Is_true_eq_true, existsb_exists in Himpl.
+    generalize dependent sol.
+    induction (premises step) as [|clause_neg_head clause_neg IHclause] ; simpl ; intros.
+    + destruct Himpl as [_ [contra _]].
+      apply contra.
+    + destruct Himpl as [x [[Heq | Hin] Hneg]].
+      * rewrite Heq, atomic_not_involution, <- atomic_not_variable_eq, Hneg.
+        reflexivity.
+      * destruct (test_atomic (atomic_not clause_neg_head) (find_value sol (var (atomic_not clause_neg_head)))) eqn:Eif ;
+        try reflexivity.
+        apply IHclause.
+        -- exists x.
+           split.
+           ++ apply Hin.
+           ++ apply Hneg.
+        -- apply Eatomic.
+  - intros Hnogood.
+    unfold satisfies_impl.
+    destruct (test_atomic_assignment (consequent step) sol) eqn:Eatomic ;
+    unfold clausal_form in Hnogood ;
+    simpl in Hnogood ;
+    unfold test_atomic_assignment in Eatomic ;
+    rewrite Eatomic in Hnogood ;
+    try reflexivity ;
+    simpl.
+    apply Is_true_eq_left, existsb_exists.
+    generalize dependent sol.
+    induction (premises step) as [|clause_neg_head clause_neg IHclause] ;
+    simpl ; intros ;
+    try contradiction.
+    destruct (test_atomic (atomic_not clause_neg_head) (find_value sol (var (atomic_not clause_neg_head)))) eqn:Eif .
+    + exists clause_neg_head.
+      split.
+      * left.
+        reflexivity.
+      * unfold test_atomic_assignment.
+        rewrite <- atomic_not_involution, atomic_not_variable_eq.
+        apply Eif.
+    + assert (Hexists: exists x : Atomic, In x clause_neg /\ negb (test_atomic_assignment x sol) = true). {
+        apply IHclause.
+        - apply Hnogood.
+        - apply Eatomic.
+      }
+      destruct Hexists as [x [Hin Hnot]].
+      exists x.
+      split.
+      * right.
+        apply Hin.
+      * apply Hnot.
+Qed.
+    
 Inductive Conclusion :=
   | unsat
   | optimal (bound : Atomic).
+
+Definition satisfies_conclusion (c : Conclusion) (sol : Assignment) :=
+  match c with
+  | unsat => false
+  | optimal bound => test_atomic_assignment bound sol
+  end.
 
 Record Proof := 
   {
