theories/ProofChecker.v
@@ -1,31 +1,128 @@
 Require Import ZArith.
 Require Import Nat.
 Require Import String.
+Require Import Bool.
+Require Import List.
 Require Import Checker.Variable.
 Require Import Checker.Atomic.
+Require Import Checker.Nogood.
 Require Import Checker.ConstraintProblem.
 Require Import Checker.Proof.
+Require Import Checker.Linear.
 
-Definition find_invalid_step 
-  (proof : Proof) (problem : ConstraintProblem) : option (nat * Step) :=
-    let 
-      var := {| 
-        name := "a"; 
-        lower_bound := 1; 
-        size := 5
-      |} 
-    in
-      Some ((Z.to_nat 5), inference nil {| var := interval var; comparator := less_equal; value := 5 |}).
+Inductive CheckerVerdict :=
+  | valid
+  | bad_step (step_index : nat) (step_def : Step)
+  | bad_conclusion.
 
-Definition is_valid_proof
-  (proof : Proof) (problem : ConstraintProblem) : Prop := True.
+Definition inc_step_index (verdict : CheckerVerdict) :=
+  match verdict with 
+  | bad_step step_index step_def => bad_step (step_index + 1) step_def
+  | _ => verdict
+end.
 
-Theorem no_invalid_step_means_proof_valid :
+Definition validate_step
+  (step : Step) (problem : ConstraintProblem) :=
+  let inference := clausal_form step in
+  match (inference_rule step) with
+  | rup_inf db => rup db inference
+  | linear constraint => linear_checker inference constraint
+  end.
+
+(* TODO How to implement the conclusion validator? *)
+Definition validate_conclusion
+  (proof_conclusion : Conclusion) (problem : ConstraintProblem) := false.
+  (* let target := match proof_conclusion with *)
+  (* | unsat => nil *)
+  (* | optimal bound => bound :: nil *)
+  (* end in *)
+  (* existsb (fun cons => Constraint.eqb cons (nogood target)) (constraints problem). *)
+
+Fixpoint validate_unpacked
+  (proof_steps : list Step) (proof_conclusion : Conclusion)
+  (problem : ConstraintProblem) : CheckerVerdict :=
+    match proof_steps with
+    | nil =>
+        if validate_conclusion proof_conclusion problem
+        then valid
+        else bad_conclusion
+    | step :: tail =>
+        if validate_step step problem
+        then
+        let problem_append :=
+        {|
+          variables := variables problem ;
+          constraints := (nogood (clausal_form step)) :: (constraints problem)
+        |} in
+        let tail_verdict := validate_unpacked tail proof_conclusion problem_append in
+        inc_step_index tail_verdict
+        else bad_step 0 step
+    end.
+
+Definition validate 
+  (proof : Proof) (problem : ConstraintProblem) : CheckerVerdict :=
+    validate_unpacked (steps proof) (conclusion proof) problem.
+  
+Definition is_valid_conclusion
+  (proof_conclusion : Conclusion) (problem : ConstraintProblem) : Prop :=
+  forall (sol : Assignment) (cons : Constraint),
+  In cons (constraints problem) ->
+  Is_true (satisfies_constraint cons sol) ->
+  Is_true (satisfies_conclusion proof_conclusion sol).
+
+Lemma unsat_no_invalid_step_implies_valid :
   forall (proof : Proof) (problem : ConstraintProblem),
-    find_invalid_step proof problem = None -> is_valid_proof proof problem.
+    conclusion proof = unsat ->
+    validate proof problem = valid ->
+    is_valid_conclusion (conclusion proof) problem.
+Proof.
+  unfold is_valid_conclusion, satisfies_conclusion, validate.
+  intros proof problem Eunsat Evalid sol cons Hin Hsat.
+  exfalso.
+  generalize dependent sol.
+  rewrite Eunsat in Evalid.
+  generalize dependent problem.
+  induction (steps proof) as [|proof_head proof_tail IHproof].
+  - (* TODO No implementation of conclusion validation yet, skipping this part for now *)
+    admit.
+  - intros.
+    simpl in Evalid.
+    destruct (validate_step proof_head problem) eqn:Evalid_step ; simpl in Evalid ; inversion Evalid as [Etail].
+    unfold inc_step_index in Etail.
+    remember 
+    {|
+      variables := variables problem ;
+      constraints := (nogood (clausal_form proof_head)) :: (constraints problem)
+    |} as problem_append eqn:Eappend.
+    destruct (validate_unpacked proof_tail unsat problem_append) eqn:Evalid_unpacked ; inversion Etail.
+    apply IHproof with (problem := problem_append) (sol := sol).
+    (* TODO This proof has to be much more elaborate, but everything short-circuits to false anyway *)
+    + apply Evalid_unpacked.
+    + rewrite Eappend.
+      simpl.
+      right.
+      apply Hin.
+    + apply Hsat.
+Admitted.
+
+Lemma bound_validate_append :
+  forall (proof : Proof) (problem : ConstraintProblem) (bound : Atomic),
+    conclusion proof = optimal bound ->
+    validate proof problem = valid ->
+    is_valid_conclusion (conclusion proof) problem.
+  Admitted.
+
+Theorem no_invalid_step_implies_valid :
+  forall (proof : Proof) (problem : ConstraintProblem),
+    validate proof problem = valid ->
+    is_valid_conclusion (conclusion proof) problem.
 Proof.
   intros.
-  unfold is_valid_proof.
-  exact I.
+  destruct (conclusion proof) eqn:Econcl ; rewrite <- Econcl.
+  + apply unsat_no_invalid_step_implies_valid.
+    - apply Econcl.
+    - apply H.
+  + apply bound_validate_append with (bound := bound).
+    - apply Econcl.
+    - apply H.
 Qed.
-
