theories/Nogood.v
@@ -12,7 +12,7 @@ Fixpoint satisfies_nogood (x : Clause) (sol : Assignment) :=
   match x with
   | nil => false
   | a :: xs =>
-let val := (find_value sol) (var a) in
+  let val := (find_value sol) (var a) in
       if test_atomic a val
       then true
       else satisfies_nogood xs sol
